theory/bpfConsistencyAux.thy
@@ -57,7 +57,7 @@ apply(rule small_steps.induct)*)
   BPF_LSH, BPF_RSH,
   BPF_ARSH 
 *)
-
+section    \<open> BPF_ALU64 \<close> 
 subsection    \<open> BPF_ALU64 auxs\<close> 
 
 lemma aluq_subgoal_rr_aux1:
@@ -107,7 +107,7 @@ lemma aluq_subgoal_rr_aux3:"op2 \<in> {BPF_SUB, BPF_MOV, BPF_ADD, BPF_AND, BPF_X
   apply(unfold eval_alu64_def,simp)
   by (unfold eval_alu64_aux1_def, simp_all)
 
-subsubsection   \<open> BPF_ALU64 ADD64\<close>  
+subsection   \<open> BPF_ALU64 ADD64\<close>  
 
 lemma addq_subgoal_rr_generic:
   assumes a0:"bins = BPF_ALU64 BPF_ADD dst (SOReg src)" and
@@ -131,7 +131,7 @@ proof -
   qed
 
 
-subsubsection   \<open> BPF_ALU64 SUB64\<close> 
+subsection   \<open> BPF_ALU64 SUB64\<close> 
 
 lemma subq_subgoal_rr_generic:
   assumes a0:"bins = BPF_ALU64 BPF_SUB dst (SOReg src)" and
@@ -154,7 +154,7 @@ proof -
     thus ?thesis using b3 by fastforce
   qed
 
-subsubsection   \<open> BPF_ALU64 AND64\<close>
+subsection   \<open> BPF_ALU64 AND64\<close>
 
 lemma andq_subgoal_rr_generic:
   assumes a0:"bins = BPF_ALU64 BPF_AND dst (SOReg src)" and
@@ -178,7 +178,7 @@ proof -
   qed
 
 
-subsubsection   \<open> BPF_ALU64 MOV64\<close>
+subsection   \<open> BPF_ALU64 MOV64\<close>
 
 lemma movq_subgoal_rr_generic:
   assumes a0:"bins = BPF_ALU64 BPF_MOV dst (SOReg src)" and
@@ -202,7 +202,7 @@ proof -
   qed
 
 
-subsubsection   \<open> BPF_ALU64 XOR64\<close>
+subsection   \<open> BPF_ALU64 XOR64\<close>
 
 lemma xorq_subgoal_rr_generic:
   assumes a0:"bins = BPF_ALU64 BPF_XOR dst (SOReg src)" and
@@ -225,7 +225,7 @@ proof -
     thus ?thesis using b3 by fastforce
   qed
 
-subsubsection   \<open> BPF_ALU64 OR64\<close> 
+subsection   \<open> BPF_ALU64 OR64\<close> 
 
 lemma orq_subgoal_rr_generic:
   assumes a0:"bins = BPF_ALU64 BPF_OR dst (SOReg src)" and
@@ -248,14 +248,14 @@ proof -
     thus ?thesis using b3 by fastforce
   qed
 
-  subsubsection   \<open> BPF_ALU64 SHL64\<close>
+subsection   \<open> BPF_ALU64 shift\<close>
 
+subsubsection   \<open> BPF_ALU64 shift auxs\<close>
 
 lemma add_sub_consistency:"add64 (Vlong a) (Vlong b) = Vlong c \<Longrightarrow> sub64 (Vlong c) (Vlong a) = (Vlong b) "
   using add64_def sub64_def by auto
 
-(*for the first step*)
-lemma interp3_aux2:
+lemma interp3_list_aux1:
   assumes a0:"xins\<noteq>[]" and 
           a1:"result = interp3 xins (Next reg m)"
         shows "result = Next reg' m' \<longrightarrow> (exec_instr (xins!0) 1 reg m) \<noteq> Stuck"
@@ -275,8 +275,7 @@ proof (rule ccontr)
    qed
  qed
 
-(*for the second step for list2 *)
-lemma interp3_aux3:
+lemma interp3_list_aux2:
   assumes a0:"length xins = (2::nat)" and 
           a1:"result = interp3 xins (Next reg m)" and
           a2:"Next reg' m' = (exec_instr (xins!0) 1 reg m)"
@@ -302,7 +301,30 @@ proof (rule ccontr)
    qed
  qed
 
-(*for the second step as a whole *)
+
+lemma interp3_list_aux3:"interp3 [] (Next reg m) = Next reg m"
+  by simp
+
+lemma interp3_length2_aux1: assumes a0:"Next reg2 m2 = interp3 xins (Next reg m)" and
+  a1:"length xins = (2::nat)"
+shows" \<exists> reg' m'. Next reg' m' = (exec_instr (xins!0) 1 reg m) \<and> Next reg2 m2 = (exec_instr (xins!1) 1 reg' m')  "
+proof-
+  from a0 a1 have "\<exists> reg' m'. Next reg' m' = (exec_instr (xins!0) 1 reg m)" 
+    by (metis interp3_list_aux1 length_0_conv outcome.exhaust zero_neq_numeral)
+  then obtain reg' m' where "Next reg' m' = (exec_instr (xins!0) 1 reg m)" by blast
+  have "\<exists> reg'' m''. Next reg'' m'' = (exec_instr (xins!1) 1 reg' m')" 
+    by (metis \<open>Next (reg'::preg \<Rightarrow> val) (m'::64 word \<Rightarrow> 8 word option option) = exec_instr ((xins::instruction list) ! (0::nat)) (1::64 word) (reg::preg \<Rightarrow> val) (m::64 word \<Rightarrow> 8 word option option)\<close> a0 a1 interp3_list_aux2 outcome.exhaust)
+  then obtain reg'' m'' where " Next reg'' m'' = (exec_instr (xins!1) 1 reg' m')"
+    by auto
+  have b4:"Next reg'' m'' = Next reg2 m2" using  a1 interp3_list_aux3
+    by (metis One_nat_def \<open>Next (reg''::preg \<Rightarrow> val) (m''::64 word \<Rightarrow> 8 word option option) = exec_instr ((xins::instruction list) ! (1::nat)) (1::64 word) (reg'::preg \<Rightarrow> val) (m'::64 word \<Rightarrow> 8 word option option)\<close> \<open>Next (reg'::preg \<Rightarrow> val) (m'::64 word \<Rightarrow> 8 word option option) = exec_instr ((xins::instruction list) ! (0::nat)) (1::64 word) (reg::preg \<Rightarrow> val) (m::64 word \<Rightarrow> 8 word option option)\<close> a0 interp3.simps(2) list_consists_2 outcome.simps(4))
+  show ?thesis using a0 a1 
+    using \<open>Next (reg''::preg \<Rightarrow> val) (m''::64 word \<Rightarrow> 8 word option option) = exec_instr ((xins::instruction list) ! (1::nat)) (1::64 word) (reg'::preg \<Rightarrow> val) (m'::64 word \<Rightarrow> 8 word option option)\<close> \<open>Next (reg'::preg \<Rightarrow> val) (m'::64 word \<Rightarrow> 8 word option option) = exec_instr ((xins::instruction list) ! (0::nat)) (1::64 word) (reg::preg \<Rightarrow> val) (m::64 word \<Rightarrow> 8 word option option)\<close> b4 by blast
+  qed
+
+lemma interp3_length2_aux2:"Next reg'' m'' = interp3 xins (Next reg m) \<Longrightarrow> length xins = (2::nat) \<Longrightarrow> \<exists> reg' m'. Next reg' m' = (exec_instr (xins!0) 1 reg m) \<and> Next reg'' m'' = (exec_instr (xins!1) 1 reg' m')  "
+  using interp3_length2_aux1 by simp
+
 lemma interp3_length4_aux1:
   assumes a0:"xins\<noteq>[]" and 
           a1:"result = interp3 xins (Next reg m)" and
@@ -329,29 +351,6 @@ proof (rule ccontr)
    qed
  qed
 
-
-
-lemma interp3_aux4:"interp3 [] (Next reg m) = Next reg m"
-  by simp
-
-lemma interp3_aux5: assumes a0:"Next reg2 m2 = interp3 xins (Next reg m)" and
-  a1:"length xins = (2::nat)"
-shows" \<exists> reg' m'. Next reg' m' = (exec_instr (xins!0) 1 reg m) \<and> Next reg2 m2 = (exec_instr (xins!1) 1 reg' m')  "
-proof-
-  from a0 a1 have "\<exists> reg' m'. Next reg' m' = (exec_instr (xins!0) 1 reg m)" 
-    by (metis interp3_aux2 length_0_conv outcome.exhaust zero_neq_numeral)
-  then obtain reg' m' where "Next reg' m' = (exec_instr (xins!0) 1 reg m)" by blast
-  have "\<exists> reg'' m''. Next reg'' m'' = (exec_instr (xins!1) 1 reg' m')" 
-    by (metis \<open>Next (reg'::preg \<Rightarrow> val) (m'::64 word \<Rightarrow> 8 word option option) = exec_instr ((xins::instruction list) ! (0::nat)) (1::64 word) (reg::preg \<Rightarrow> val) (m::64 word \<Rightarrow> 8 word option option)\<close> a0 a1 interp3_aux3 outcome.exhaust)
-  then obtain reg'' m'' where " Next reg'' m'' = (exec_instr (xins!1) 1 reg' m')"
-    by auto
-  have b4:"Next reg'' m'' = Next reg2 m2" using interp3_aux4 a1 
-    by (metis One_nat_def \<open>Next (reg''::preg \<Rightarrow> val) (m''::64 word \<Rightarrow> 8 word option option) = exec_instr ((xins::instruction list) ! (1::nat)) (1::64 word) (reg'::preg \<Rightarrow> val) (m'::64 word \<Rightarrow> 8 word option option)\<close> \<open>Next (reg'::preg \<Rightarrow> val) (m'::64 word \<Rightarrow> 8 word option option) = exec_instr ((xins::instruction list) ! (0::nat)) (1::64 word) (reg::preg \<Rightarrow> val) (m::64 word \<Rightarrow> 8 word option option)\<close> a0 interp3.simps(2) list_consists_2 outcome.simps(4))
-  show ?thesis using a0 a1 
-    using \<open>Next (reg''::preg \<Rightarrow> val) (m''::64 word \<Rightarrow> 8 word option option) = exec_instr ((xins::instruction list) ! (1::nat)) (1::64 word) (reg'::preg \<Rightarrow> val) (m'::64 word \<Rightarrow> 8 word option option)\<close> \<open>Next (reg'::preg \<Rightarrow> val) (m'::64 word \<Rightarrow> 8 word option option) = exec_instr ((xins::instruction list) ! (0::nat)) (1::64 word) (reg::preg \<Rightarrow> val) (m::64 word \<Rightarrow> 8 word option option)\<close> b4 by blast
-  qed
-
-(*for the third step as for list4 *)
 lemma interp3_length4_aux2:
   assumes a0:"length xins = (4::nat)" and 
           a1:"result = interp3 xins (Next reg m)" and
@@ -373,7 +372,7 @@ proof (rule ccontr)
        by (metis One_nat_def Suc_1 a0 append_Nil less_1_mult less_2_cases_iff numeral_Bit0_eq_double take_0 take_Suc_conv_app_nth zero_less_numeral)
      have b2_2:"length ?tmplist = (2::nat)" 
        by (simp add: b2_1)
-     have b2_3:"\<exists> reg1 m1. Next reg1 m1 = (exec_instr (xins!0) 1 reg m) \<and> Next reg2 m2 = (exec_instr (xins!1) 1 reg1 m1 )" using a2 b2_2 b2_1 interp3_aux5 
+     have b2_3:"\<exists> reg1 m1. Next reg1 m1 = (exec_instr (xins!0) 1 reg m) \<and> Next reg2 m2 = (exec_instr (xins!1) 1 reg1 m1 )" using a2 b2_2 b2_1 interp3_length2_aux1 
        by (metis Cons_eq_appendI One_nat_def append_Nil assms(3) nth_Cons_0 nth_Cons_Suc)
      then obtain reg1 m1 where b2_4:"Next reg1 m1 = (exec_instr (xins!0) 1 reg m) \<and> Next reg2 m2 = (exec_instr (xins!1) 1 reg1 m1 )" by auto
      have b2_5:"Next reg1 m1 = (exec_instr (xins!0) 1 reg m)" using b2_3 using b2_4 by blast
@@ -390,34 +389,6 @@ proof (rule ccontr)
        using a1 a4 by (simp add: a0 exec_instr_def)
    qed
  qed
-
-lemma interp3_length4_aux5:
-  assumes a0:"length xins = (4::nat)" and 
-    a1:"Next reg'' m'' = interp3 xins (Next reg m)" and
-    a2:"Next reg' m' = (exec_instr (xins!0) 1 reg m)"
-  shows "\<exists> reg2 m2. interp3 (butlast(tl xins)) (Next reg' m') = Next reg2 m2"
-  sorry
-(*proof -
-     have b1:"(take 2 xins) @ (drop 2 xins)= xins" using a0
-       by (simp add: Cons_nth_drop_Suc numeral_3_eq_3 numeral_nat(2))
-     let ?tmplist = "take 2 xins"
-     have b2_1:"?tmplist = [(xins!0)]@[(xins!1)]" 
-       by (metis One_nat_def Suc_1 a0 append_Nil less_1_mult less_2_cases_iff numeral_Bit0_eq_double take_0 take_Suc_conv_app_nth zero_less_numeral)
-     have b2_2:"length ?tmplist = (2::nat)" 
-       by (simp add: b2_1)
-     have b2_3:"\<exists> reg1 m1. Next reg1 m1 = (exec_instr (xins!0) 1 reg m) \<and> Next reg2 m2 = (exec_instr (xins!1) 1 reg1 m1 )" using a2 b2_2 b2_1 interp3_aux5 
-       by (metis Cons_eq_appendI One_nat_def append_Nil assms(3) nth_Cons_0 nth_Cons_Suc)
-     then obtain reg1 m1 where b2_4:"Next reg1 m1 = (exec_instr (xins!0) 1 reg m) \<and> Next reg2 m2 = (exec_instr (xins!1) 1 reg1 m1 )" by auto
-     have b2_5:"Next reg1 m1 = (exec_instr (xins!0) 1 reg m)" using b2_3 using b2_4 by blast
-     have b2_6:" Next reg2 m2 = (exec_instr (xins!1) 1 reg1 m1 )" using b2_3 using b2_4 by blast
-     have b2_7:"[xins!0]@[xins!1] @ (drop 2 xins)= xins" using a0
-       by (simp add: Cons_nth_drop_Suc numeral_3_eq_3 numeral_nat(2))
-     have b2:"interp3 (drop 2 xins) (Next reg2 m2) = interp3 (xins) (Next reg m)" using a0 a1 a2 a3 b0 
-       using append_Cons append_Nil assms(3) b2_5 b2_6 b2_7 interp3.simps(2) outcome.simps(4) by metis
-     thus ?thesis by simp
- qed
-*)
-
 
 lemma interp3_length4_aux3:
   assumes a0:"length xins = (4::nat)" and 
@@ -441,7 +412,7 @@ proof (rule ccontr)
      let ?tmplist = "(butlast xins)"
      have b2_1:"?tmplist = [(?tmplist!0)]@(tl ?tmplist)" using b1_2 by simp
      have b2_2:"length ?tmplist > 0" using b2_1 by fastforce
-     have b2_3:"\<exists> reg1 m1. Next reg1 m1 = (exec_instr (xins!0) 1 reg m)" using b1_3 interp3_aux2 
+     have b2_3:"\<exists> reg1 m1. Next reg1 m1 = (exec_instr (xins!0) 1 reg m)" using b1_3 interp3_list_aux1 
        by (metis a1 a4 bot_nat_0.extremum_strict list.size(3) outcome.exhaust)
      have b2_4:"(?tmplist!0) = (xins!0)" using b2_2 nth_butlast by blast
      have b2_5:"\<exists> reg1 m1. Next reg1 m1 = (exec_instr (?tmplist!0) 1 reg m) \<and> Next reg3 m3 = interp3 (tl ?tmplist) (Next reg1 m1) " 
@@ -453,9 +424,9 @@ proof (rule ccontr)
      have b3_1:"?tmplist2 = tl ?tmplist" by (simp add: b1_2)
      have b3_2:"Next reg3 m3 = interp3 (?tmplist2) (Next reg1 m1)" using b2_4 b3_1 by simp
      have b3_3:"\<exists> reg2 m2. Next reg2 m2 = (exec_instr (?tmplist2!0) 1 reg1 m1) \<and> Next reg3 m3 = (exec_instr (?tmplist2!1) 1 reg2 m2)" 
-       using a2 b2_2 b2_1 interp3_aux5 b3_1 b3_2 b3_0 by blast
+       using a2 b2_2 b2_1 interp3_length2_aux1 b3_1 b3_2 b3_0 by blast
      have b2:"(exec_instr (last xins) 1 reg3 m3)  = interp3 (xins) (Next reg m)" using a0 a1 a2 a3 b0 
-       by (smt (z3) Suc_eq_plus1 add_2_eq_Suc append_Cons append_Nil b1_2 b2_4 b3_0 b3_1 diff_Suc_1' interp3.simps(2) interp3_aux3 interp3_aux5 last_conv_nth last_tl length_0_conv length_Suc_conv list.sel(3) list.simps(3) list.size(3) list_consists_4 nth_Cons_0 outcome.case(1) outcome.inject zero_neq_numeral)
+       by (smt (z3) Suc_eq_plus1 add_2_eq_Suc append_Cons append_Nil b1_2 b2_4 b3_0 b3_1 diff_Suc_1' interp3.simps(2) interp3_list_aux2 interp3_length2_aux1 last_conv_nth last_tl length_0_conv length_Suc_conv list.sel(3) list.simps(3) list.size(3) list_consists_4 nth_Cons_0 outcome.case(1) outcome.inject zero_neq_numeral)
      have b3: "(exec_instr (last xins) 1 reg3 m3)  = Stuck"using a0 b0 exec_instr_def a2
        using interp2.elims nth_Cons_0 outcome.case(2) outcome.simps(4) by auto
      have b4: "interp3 xins (Next reg m) = Stuck" using a0 a1 b3 exec_instr_def a2 
@@ -465,8 +436,7 @@ proof (rule ccontr)
    qed
  qed
 
-
-lemma interp3_length4_aux6:
+lemma interp3_length4_aux4:
   assumes a0:"length xins = (4::nat)" and 
           a1:"Next reg'' m''= interp3 xins (Next reg m)" 
         shows "\<exists> reg' m'. Next reg' m' = interp3 (take 2 xins) (Next reg m) \<and> Next reg'' m'' = interp3 (drop 2 xins) (Next reg' m')"
@@ -476,18 +446,18 @@ proof-
      have b1_2: "(butlast xins) = [xins!0]@[xins!1]@[xins!2]" using b1_1 a0 
        by (metis One_nat_def append_Cons append_Nil butlast.simps(2) list.simps(3) list_consists_4)
      have b1_3:"length xins >0" using a0 by simp
-     have b2_3:"\<exists> reg1 m1. Next reg1 m1 = (exec_instr (xins!0) 1 reg m)" using b1_3 interp3_aux2 
+     have b2_3:"\<exists> reg1 m1. Next reg1 m1 = (exec_instr (xins!0) 1 reg m)" using b1_3 interp3_list_aux1 
        by (metis a1 bot_nat_0.extremum_strict list.size(3) outcome.exhaust)
      have b2_5:"\<exists> reg1 m1. Next reg1 m1 = (exec_instr (xins!0) 1 reg m) \<and> Next reg'' m'' = interp3 (tl xins) (Next reg1 m1) " 
        using a1
        by (metis b1_3 b2_3 interp3.elims length_greater_0_conv list.sel(3) nth_Cons_0 outcome.case(1))
      then obtain reg1 m1 where b2_6:" Next reg1 m1 = (exec_instr (xins!0) 1 reg m) \<and> Next reg'' m'' = interp3 (tl xins) (Next reg1 m1)" by auto
      have b3_3:"\<exists> reg2 m2. Next reg2 m2 = (exec_instr (xins!1) 1 reg1 m1)"using exec_instr_def a0 
-       by (metis (no_types, opaque_lifting) Suc_eq_plus1 add.commute add.right_neutral b2_6 diff_Suc_1' interp3_aux2 list.sel(3) list_consists_4 neq_Nil_conv nth_Cons_numeral numeral_eq_one_iff outcome.exhaust)
+       by (metis (no_types, opaque_lifting) Suc_eq_plus1 add.commute add.right_neutral b2_6 diff_Suc_1' interp3_list_aux1 list.sel(3) list_consists_4 neq_Nil_conv nth_Cons_numeral numeral_eq_one_iff outcome.exhaust)
      then obtain reg2 m2 where b3_4:"Next reg2 m2 = (exec_instr (xins!1) 1 reg1 m1)" by auto
      have b4_1:"take 2 xins = [xins!0]@[xins!1]" by (simp add: a0 numeral_2_eq_2 take_Suc_conv_app_nth)
      have b4:"Next reg2 m2 = interp3 (take 2 xins) (Next reg m)" using a0 b3_4 b4_1 b2_6 
-       by (metis append_Cons append_Nil interp3.simps(2) interp3_aux4 outcome.case(1))
+       by (metis append_Cons append_Nil interp3.simps(2) interp3_list_aux3 outcome.case(1))
      have b5_1:"[xins!0]@[xins!1] @ (drop 2 xins)= xins" using a0
        by (simp add: Cons_nth_drop_Suc numeral_3_eq_3 numeral_nat(2))
      have b5_2:"interp3 (drop 2 xins) (Next reg2 m2) = interp3 (xins) (Next reg m)" using a0 a1 b5_1 b4
@@ -497,7 +467,34 @@ proof-
      thus ?thesis by fastforce
    qed
 
-lemma interp3_length4_aux4:
+lemma interp3_length4_aux5:
+  assumes a0:"length xins = (4::nat)" and 
+    a1:"Next reg'' m'' = interp3 xins (Next reg m)" and
+    a2:"Next reg' m' = (exec_instr (xins!0) 1 reg m)"
+  shows "\<exists> reg2 m2. interp3 (butlast(tl xins)) (Next reg' m') = Next reg2 m2"
+  sorry
+(*proof -
+     have b1:"(take 2 xins) @ (drop 2 xins)= xins" using a0
+       by (simp add: Cons_nth_drop_Suc numeral_3_eq_3 numeral_nat(2))
+     let ?tmplist = "take 2 xins"
+     have b2_1:"?tmplist = [(xins!0)]@[(xins!1)]" 
+       by (metis One_nat_def Suc_1 a0 append_Nil less_1_mult less_2_cases_iff numeral_Bit0_eq_double take_0 take_Suc_conv_app_nth zero_less_numeral)
+     have b2_2:"length ?tmplist = (2::nat)" 
+       by (simp add: b2_1)
+     have b2_3:"\<exists> reg1 m1. Next reg1 m1 = (exec_instr (xins!0) 1 reg m) \<and> Next reg2 m2 = (exec_instr (xins!1) 1 reg1 m1 )" using a2 b2_2 b2_1 interp3_length2_aux1 
+       by (metis Cons_eq_appendI One_nat_def append_Nil assms(3) nth_Cons_0 nth_Cons_Suc)
+     then obtain reg1 m1 where b2_4:"Next reg1 m1 = (exec_instr (xins!0) 1 reg m) \<and> Next reg2 m2 = (exec_instr (xins!1) 1 reg1 m1 )" by auto
+     have b2_5:"Next reg1 m1 = (exec_instr (xins!0) 1 reg m)" using b2_3 using b2_4 by blast
+     have b2_6:" Next reg2 m2 = (exec_instr (xins!1) 1 reg1 m1 )" using b2_3 using b2_4 by blast
+     have b2_7:"[xins!0]@[xins!1] @ (drop 2 xins)= xins" using a0
+       by (simp add: Cons_nth_drop_Suc numeral_3_eq_3 numeral_nat(2))
+     have b2:"interp3 (drop 2 xins) (Next reg2 m2) = interp3 (xins) (Next reg m)" using a0 a1 a2 a3 b0 
+       using append_Cons append_Nil assms(3) b2_5 b2_6 b2_7 interp3.simps(2) outcome.simps(4) by metis
+     thus ?thesis by simp
+ qed
+*)
+
+lemma interp3_length4_aux6:
   assumes a0:"length xins = (4::nat)" and 
           a1:"Next reg'' m''= interp3 xins (Next reg m)" 
         shows "\<exists> reg' m'. Next reg' m' = interp3 (butlast xins) (Next reg m) \<and> Next reg'' m'' = (exec_instr (last xins) 1 reg' m')"
@@ -507,18 +504,18 @@ proof-
      have b1_2: "(butlast xins) = [xins!0]@[xins!1]@[xins!2]" using b1_1 a0 
        by (metis One_nat_def append_Cons append_Nil butlast.simps(2) list.simps(3) list_consists_4)
      have b1_3:"length xins >0" using a0 by simp
-     have b2_3:"\<exists> reg1 m1. Next reg1 m1 = (exec_instr (xins!0) 1 reg m)" using b1_3 interp3_aux2 
+     have b2_3:"\<exists> reg1 m1. Next reg1 m1 = (exec_instr (xins!0) 1 reg m)" using b1_3 interp3_list_aux1 
        by (metis a1 bot_nat_0.extremum_strict list.size(3) outcome.exhaust)
      have b2_5:"\<exists> reg1 m1. Next reg1 m1 = (exec_instr (xins!0) 1 reg m) \<and> Next reg'' m'' = interp3 (tl xins) (Next reg1 m1) " 
        using a1
        by (metis b1_3 b2_3 interp3.elims length_greater_0_conv list.sel(3) nth_Cons_0 outcome.case(1))
      then obtain reg1 m1 where b2_6:" Next reg1 m1 = (exec_instr (xins!0) 1 reg m) \<and> Next reg'' m'' = interp3 (tl xins) (Next reg1 m1)" by auto
      have b3_3:"\<exists> reg2 m2. Next reg2 m2 = (exec_instr (xins!1) 1 reg1 m1)"using exec_instr_def a0 
-       by (metis (no_types, opaque_lifting) Suc_eq_plus1 add.commute add.right_neutral b2_6 diff_Suc_1' interp3_aux2 list.sel(3) list_consists_4 neq_Nil_conv nth_Cons_numeral numeral_eq_one_iff outcome.exhaust)
+       by (metis (no_types, opaque_lifting) Suc_eq_plus1 add.commute add.right_neutral b2_6 diff_Suc_1' interp3_list_aux1 list.sel(3) list_consists_4 neq_Nil_conv nth_Cons_numeral numeral_eq_one_iff outcome.exhaust)
      then obtain reg2 m2 where b3_4:"Next reg2 m2 = (exec_instr (xins!1) 1 reg1 m1)" by auto
      have b4_1:"take 2 xins = [xins!0]@[xins!1]" by (simp add: a0 numeral_2_eq_2 take_Suc_conv_app_nth)
      have b4:"Next reg2 m2 = interp3 (take 2 xins) (Next reg m)" using a0 b3_4 b4_1 b2_6 
-       by (metis append_Cons append_Nil interp3.simps(2) interp3_aux4 outcome.case(1))
+       by (metis append_Cons append_Nil interp3.simps(2) interp3_list_aux3 outcome.case(1))
      have b5_1:"[xins!0]@[xins!1] @ (drop 2 xins)= xins" using a0
        by (simp add: Cons_nth_drop_Suc numeral_3_eq_3 numeral_nat(2))
      have b5_2:"interp3 (drop 2 xins) (Next reg2 m2) = interp3 (xins) (Next reg m)" using a0 a1 b5_1 b4
@@ -527,91 +524,20 @@ proof-
        using b5_2 b4 using a1 by force
      then obtain reg2 m2 where b5:"Next reg2 m2 = interp3 (take 2 xins) (Next reg m) \<and> Next reg'' m'' = interp3 (drop 2 xins) (Next reg2 m2)" by auto
      have b6_1:"\<exists> reg3 m3. Next reg3 m3 = (exec_instr (xins!2) 1 reg2 m2) " using b5 a0 a1 
-       by (metis One_nat_def Suc_1 append_Cons append_Nil b1_2 b5_1 butlast.simps(2) interp3_aux2 list.simps(3) nth_Cons_Suc outcome.exhaust)
+       by (metis One_nat_def Suc_1 append_Cons append_Nil b1_2 b5_1 butlast.simps(2) interp3_list_aux1 list.simps(3) nth_Cons_Suc outcome.exhaust)
      then obtain reg3 m3 where b6_2:"Next reg3 m3 = (exec_instr (xins!2) 1 reg2 m2)" by auto
      have b6_3:"take 3 xins = [xins!0]@[xins!1]@[xins!2]" using a0 
        by (simp add: One_nat_def Suc_1 add_One numeral_3_eq_3 numeral_nat(2) take_Suc_conv_app_nth)
      have b6_3:"Next reg3 m3 = interp3 (take 3 xins) (Next reg m)" using a0 b5 b6_2 b6_3 
-       by (metis (no_types, lifting) append_Cons append_Nil b2_6 b3_4 b4 interp3.simps(2) interp3_aux4 outcome.case(1))
+       by (metis (no_types, lifting) append_Cons append_Nil b2_6 b3_4 b4 interp3.simps(2) interp3_list_aux3 outcome.case(1))
      have b6_4:"[xins!0]@[xins!1]@[xins!2]@[last xins] = xins"
        using append_butlast_last_id b1_2 b1_3 by fastforce
      have b6_5:"butlast xins = take 3 xins" using a0
        by (metis Suc_length_conv append_Cons append_Nil b1_2 butlast_conv_take length_butlast list.size(3) numeral_3_eq_3)
      have b6:"Next reg3 m3 = interp3 (take 3 xins) (Next reg m) \<and> Next reg'' m'' = (exec_instr (last xins) 1 reg3 m3)" using a0 b6_3 b6_4 b5 b5_1 b6_2 
-       by (smt (verit, del_insts) Cons_eq_appendI One_nat_def Suc_length_conv eq_Nil_appendI interp3_aux5 list.size(3) nth_Cons_0 nth_Cons_Suc numeral_2_eq_2 outcome.inject same_append_eq)     
+       by (smt (verit, del_insts) Cons_eq_appendI One_nat_def Suc_length_conv eq_Nil_appendI interp3_length2_aux1 list.size(3) nth_Cons_0 nth_Cons_Suc numeral_2_eq_2 outcome.inject same_append_eq)     
      thus ?thesis using b6 b6_5 by auto
    qed
-
-
-lemma shift_subgoal_rr_aux1_1:"Next reg'' m'' = interp3 xins (Next reg m) \<Longrightarrow> length xins = (2::nat) \<Longrightarrow> \<exists> reg' m'. Next reg' m' = (exec_instr (xins!0) 1 reg m) \<and> Next reg'' m'' = (exec_instr (xins!1) 1 reg' m')  "
-  using interp3_aux5 by simp
-
-lemma shift_subgoal_rr_aux2_1:"xins = Pmovq_rr (x64Syntax.RCX) src  \<Longrightarrow> 
-    Next reg'' m'' = (exec_instr xins 1 reg m) \<Longrightarrow> m'' = m "
-  apply(unfold exec_instr_def) by simp
-
-lemma shift_subgoal_rr_aux2_2:"xins = Pshlq_r dst \<Longrightarrow> 
-    Next reg'' m'' = (exec_instr xins 1 reg m) \<Longrightarrow> m'' = m"
-  apply(unfold exec_instr_def) by simp
-
-lemma shift_subgoal_rr_aux2_3:
-  assumes a0:"xins = [(Pmovq_rr (x64Syntax.RCX) src),(Pshlq_r dst)]" and 
-    a1:"Next reg' m' = (exec_instr (xins!0) 1 reg m) " and
-    a2:"Next reg'' m'' = (exec_instr (xins!1) 1 reg' m') " 
-  shows " m'' = m"
-  using shift_subgoal_rr_aux2_1 shift_subgoal_rr_aux2_2 
-  by (metis One_nat_def a0 a1 a2 nth_Cons_0 nth_Cons_Suc)
-
-lemma shift_subgoal_rr_aux2:
-  assumes a0:"xins = [(Pmovq_rr (x64Syntax.RCX) src),(Pshlq_r dst)]" and 
-    a1:"Next reg'' m'' = interp3 xins (Next reg m) " 
-  shows " m'' = m"
-proof-
-  have b0:"length xins = (2::nat)" using a0 by simp
-  thus ?thesis using b0 a0 a1 shift_subgoal_rr_aux2_3 
-    by (meson shift_subgoal_rr_aux1_1)
-qed
-
-lemma reg_rsp_consist:"r = (bpf_to_x64_reg dst) \<Longrightarrow> r \<noteq> x64Syntax.RSP"
-  apply(cases dst) 
-  by (unfold bpf_to_x64_reg_corr bpf_to_x64_reg_def, simp_all)
-
-lemma shift_subgoal_rr_aux3_1:"xins = Pmovq_rr (x64Syntax.RCX) (bpf_to_x64_reg src)\<Longrightarrow> 
-    Next reg'' m'' = (exec_instr xins 1 reg m) \<Longrightarrow> reg'' (IR SP) = reg (IR SP) "
-  apply(unfold exec_instr_def reg_rsp_consist bpf_to_x64_reg_corr) 
-  using nextinstr_def reg_rsp_consist by fastforce
-
-lemma shift_subgoal_rr_aux3_2:"xins = Pshlq_r (bpf_to_x64_reg dst) \<Longrightarrow> 
-    Next reg'' m'' = (exec_instr xins 1 reg m) \<Longrightarrow> reg'' (IR SP) = reg (IR SP) "
-  apply(unfold exec_instr_def reg_rsp_consist bpf_to_x64_reg_corr)
-  apply(cases xins, simp_all)
-  apply(unfold nextinstr_def reg_rsp_consist shl64_def nextinstr_nf_def reg_rsp_consist)
-  apply(cases "reg (IR (bpf_to_x64_reg dst))",simp_all)
-      apply metis
-  subgoal for x2 apply (simp add:add64_def)sorry
-  subgoal for x3 apply (simp add:add64_def) sorry
-  subgoal for x4 apply (simp add:add64_def) sorry
-  subgoal for x5 apply (simp add:add64_def) 
-    using reg_rsp_consist by blast
-  (* no dealing with Vundef ? *)
-  done
-lemma shift_subgoal_rr_aux3_3:
-  assumes a0:"xins = [(Pmovq_rr (x64Syntax.RCX)(bpf_to_x64_reg src)),(Pshlq_r (bpf_to_x64_reg dst))]" and 
-    a1:"Next reg' m' = (exec_instr (xins!0) 1 reg m) " and
-    a2:"Next reg'' m'' = (exec_instr (xins!1) 1 reg' m') " 
-  shows " reg'' (IR SP) = reg (IR SP) "
-  using shift_subgoal_rr_aux3_1 shift_subgoal_rr_aux3_2 reg_rsp_consist
-  by (metis One_nat_def a0 a1 a2 nth_Cons_0 nth_Cons_Suc)
-
-lemma shift_subgoal_rr_aux3:
-  assumes a0:"xins = [(Pmovq_rr (x64Syntax.RCX)(bpf_to_x64_reg src)),(Pshlq_r (bpf_to_x64_reg dst))]" and 
-    a1:"Next reg'' m'' = interp3 xins (Next reg m) " 
-  shows "reg'' (IR SP) = reg (IR SP)"
-proof-
-  have b0:"length xins = (2::nat)" using a0 by simp
-  thus ?thesis using b0 a0 a1 shift_subgoal_rr_aux3_3 
-    by (meson shift_subgoal_rr_aux1_1)
-qed
 
 lemma push_pop_subgoal_rr_aux1:
   assumes a0:"hd xins = Ppushl_r x64Syntax.RCX" and 
@@ -675,7 +601,7 @@ lemma push_pop_subgoal_rr_aux2_2:
   shows "reg'' (IR x64Syntax.RCX) = reg (IR x64Syntax.RCX)"
 proof-
   have b0:"length xins = (2::nat)" using a0 by simp
-  thus ?thesis using b0 a0 a1 push_pop_subgoal_rr_aux2_1 shift_subgoal_rr_aux1_1
+  thus ?thesis using b0 a0 a1 push_pop_subgoal_rr_aux2_1 interp3_length2_aux2
     by metis
 qed
 
@@ -684,7 +610,6 @@ lemma push_pop_subgoal_rr_aux2_3:
           a1:"last xins = Ppopl x64Syntax.RCX"and
           a2:"interp3 (butlast(tl xins)) (Next reg' m') = Next reg2 m'"and
           a3:"Next reg'' m'' = (exec_instr (last xins) 1 reg2 m') " and
-          (*a3:"Next reg'' m'' = interp3 xins (Next reg m)" and*)
           a5:"Next reg' m' = (exec_instr (xins!0) 1 reg m) " and
           a6:"reg' (IR SP) =  reg2 (IR SP)"
   shows "reg'' (IR x64Syntax.RCX) = reg (IR x64Syntax.RCX)"
@@ -695,7 +620,6 @@ proof-
   have b0:"Next reg' m' = exec_push 1 M32 m reg (reg (IR x64Syntax.RCX))" using exec_instr_def a0 
     using exec_push_def a5 a0 
     by (smt (z3) a1 hd_Nil_eq_last hd_conv_nth instruction.distinct(5787) instruction.simps(6295))
-  (*then obtain reg' m' where b0:"Next reg' m' = exec_push 1 M32 m reg (reg (IR x64Syntax.RCX))" by blast*)
   have b1:"Next reg' m' =
     (case storev M32 m (sub64 (reg (IR SP)) (vlong_of_memory_chunk M32)) (reg (IR ireg.RCX)) of None \<Rightarrow> Stuck
      | Some (x::64 word \<Rightarrow> 8 word option option) \<Rightarrow>
@@ -729,15 +653,77 @@ proof-
   thus ?thesis using c4 by simp
 qed
 
+lemma reg_rsp_consist:"r = (bpf_to_x64_reg dst) \<Longrightarrow> r \<noteq> x64Syntax.RSP"
+  apply(cases dst) 
+  by (unfold bpf_to_x64_reg_corr bpf_to_x64_reg_def, simp_all)
 
-(*lemma hh2: assumes a0:"Next reg'' m'' = interp3 xins (Next reg m)" and
-  a1:"length xins \<ge> (2::nat)" and
-  a2:"length xins \<ge> (2::nat)"
-shows" \<exists> reg' m'. Next reg' m' = interp3 (butlast xins) (Next reg m) \<and> Next reg'' m'' = (exec_instr (last xins) 1 reg' m')   "
-  sorry
-*)
 
-lemma shift_subgoal_rr_aux4_1:
+subsubsection   \<open> BPF_ALU64 LSH aux\<close>
+
+lemma shl_subgoal_rr_aux2_1:"xins = Pmovq_rr (x64Syntax.RCX) src  \<Longrightarrow> 
+    Next reg'' m'' = (exec_instr xins 1 reg m) \<Longrightarrow> m'' = m "
+  apply(unfold exec_instr_def) by simp
+
+lemma shl_subgoal_rr_aux2_2:"xins = Pshlq_r dst \<Longrightarrow> 
+    Next reg'' m'' = (exec_instr xins 1 reg m) \<Longrightarrow> m'' = m"
+  apply(unfold exec_instr_def) by simp
+
+lemma shl_subgoal_rr_aux2_3:
+  assumes a0:"xins = [(Pmovq_rr (x64Syntax.RCX) src),(Pshlq_r dst)]" and 
+    a1:"Next reg' m' = (exec_instr (xins!0) 1 reg m) " and
+    a2:"Next reg'' m'' = (exec_instr (xins!1) 1 reg' m') " 
+  shows " m'' = m"
+  using shl_subgoal_rr_aux2_1 shl_subgoal_rr_aux2_2 
+  by (metis One_nat_def a0 a1 a2 nth_Cons_0 nth_Cons_Suc)
+
+lemma shl_subgoal_rr_aux2:
+  assumes a0:"xins = [(Pmovq_rr (x64Syntax.RCX) src),(Pshlq_r dst)]" and 
+    a1:"Next reg'' m'' = interp3 xins (Next reg m) " 
+  shows " m'' = m"
+proof-
+  have b0:"length xins = (2::nat)" using a0 by simp
+  thus ?thesis using b0 a0 a1 shl_subgoal_rr_aux2_3 
+    by (meson interp3_length2_aux2)
+qed
+
+lemma shl_subgoal_rr_aux3_1:"xins = Pmovq_rr (x64Syntax.RCX) (bpf_to_x64_reg src)\<Longrightarrow> 
+    Next reg'' m'' = (exec_instr xins 1 reg m) \<Longrightarrow> reg'' (IR SP) = reg (IR SP) "
+  apply(unfold exec_instr_def reg_rsp_consist bpf_to_x64_reg_corr) 
+  using nextinstr_def reg_rsp_consist by fastforce
+
+lemma shl_subgoal_rr_aux3_2:"xins = Pshlq_r (bpf_to_x64_reg dst) \<Longrightarrow> 
+    Next reg'' m'' = (exec_instr xins 1 reg m) \<Longrightarrow> reg'' (IR SP) = reg (IR SP) "
+  apply(unfold exec_instr_def reg_rsp_consist bpf_to_x64_reg_corr)
+  apply(cases xins, simp_all)
+  apply(unfold nextinstr_def reg_rsp_consist shl64_def nextinstr_nf_def reg_rsp_consist)
+  apply(cases "reg (IR (bpf_to_x64_reg dst))",simp_all)
+      apply metis
+  subgoal for x2 apply (simp add:add64_def)sorry
+  subgoal for x3 apply (simp add:add64_def) sorry
+  subgoal for x4 apply (simp add:add64_def) sorry
+  subgoal for x5 apply (simp add:add64_def) 
+    using reg_rsp_consist by blast
+  (* no dealing with VByte conversion *)
+  done
+lemma shl_subgoal_rr_aux3_3:
+  assumes a0:"xins = [(Pmovq_rr (x64Syntax.RCX)(bpf_to_x64_reg src)),(Pshlq_r (bpf_to_x64_reg dst))]" and 
+    a1:"Next reg' m' = (exec_instr (xins!0) 1 reg m) " and
+    a2:"Next reg'' m'' = (exec_instr (xins!1) 1 reg' m') " 
+  shows " reg'' (IR SP) = reg (IR SP) "
+  using shl_subgoal_rr_aux3_1 shl_subgoal_rr_aux3_2 reg_rsp_consist
+  by (metis One_nat_def a0 a1 a2 nth_Cons_0 nth_Cons_Suc)
+
+lemma shl_subgoal_rr_aux3:
+  assumes a0:"xins = [(Pmovq_rr (x64Syntax.RCX)(bpf_to_x64_reg src)),(Pshlq_r (bpf_to_x64_reg dst))]" and 
+    a1:"Next reg'' m'' = interp3 xins (Next reg m) " 
+  shows "reg'' (IR SP) = reg (IR SP)"
+proof-
+  have b0:"length xins = (2::nat)" using a0 by simp
+  thus ?thesis using b0 a0 a1 shl_subgoal_rr_aux3_3 
+    by (meson interp3_length2_aux2)
+qed
+
+lemma shl_subgoal_rr_aux4_1:
   assumes a0:"xins = [Ppushl_r x64Syntax.RCX, Pmovq_rr (x64Syntax.RCX) (bpf_to_x64_reg src),Pshlq_r (bpf_to_x64_reg dst),Ppopl x64Syntax.RCX]" and 
     a1:"Next reg'' m'' = interp3 xins (Next reg m)" 
   shows "reg'' (IR x64Syntax.RCX) = reg (IR x64Syntax.RCX)"
@@ -755,8 +741,8 @@ proof-
     by (simp add: a0 b0 exec_instr_def)
   have b2:"\<exists> reg2 m2. interp3 ?midlist (Next reg' m') = Next reg2 m2" using interp3_length4_aux5 b1 a0 a1 b2_0 b0 b2_1 by fastforce
   then obtain reg2 m2 where b3:"interp3 ?midlist (Next reg' m') = Next reg2 m2" by auto
-  have b4:"m2 = m'" using shift_subgoal_rr_aux2 by (metis b3)
-  have b5:"reg' (IR SP) =  reg2 (IR SP)" using shift_subgoal_rr_aux3 b3 by metis
+  have b4:"m2 = m'" using shl_subgoal_rr_aux2 by (metis b3)
+  have b5:"reg' (IR SP) =  reg2 (IR SP)" using shl_subgoal_rr_aux3 b3 by metis
   have b6:"Next reg' m' = (exec_instr (xins!0) 1 reg m) " using a0 by (simp add: b0 exec_instr_def)
   have b7_1:"length xins \<ge> (2::nat)" using a0 by simp
   have b7_2:"Next reg2 m2 = interp3 (butlast xins) (Next reg m)" using b3 b0 a0 by (simp add: b6)
@@ -766,7 +752,7 @@ proof-
     by (metis a0 b3 butlast.simps(2) list.distinct(1) list.sel(3))
 qed
 
-lemma shift_subgoal_rr_aux4_2:"xins = Pmovq_rr (x64Syntax.RCX) src \<Longrightarrow> 
+lemma shl_subgoal_rr_aux4_2:"xins = Pmovq_rr (x64Syntax.RCX) src \<Longrightarrow> 
     Next reg' m' = (exec_instr xins 1 reg m)\<Longrightarrow> 
     \<forall> r . r \<noteq> x64Syntax.RCX \<longrightarrow> reg' (IR r) = reg (IR r)"
   apply(unfold exec_instr_def )
@@ -774,7 +760,7 @@ lemma shift_subgoal_rr_aux4_2:"xins = Pmovq_rr (x64Syntax.RCX) src \<Longrightar
   apply(unfold nextinstr_nf_def nextinstr_def add64_def)
   by auto
 
-lemma  shift_subgoal_rr_aux4_3:"xins = Pmovq_rr (x64Syntax.RCX) (bpf_to_x64_reg src) \<Longrightarrow> 
+lemma  shl_subgoal_rr_aux4_3:"xins = Pmovq_rr (x64Syntax.RCX) (bpf_to_x64_reg src) \<Longrightarrow> 
     Next reg' m' = (exec_instr xins 1 reg m)\<Longrightarrow> 
     \<forall> r. bpf_to_x64_reg r \<noteq> x64Syntax.RCX \<longrightarrow> reg' (IR (bpf_to_x64_reg r)) = reg (IR (bpf_to_x64_reg r))"
   apply(unfold exec_instr_def )
@@ -782,7 +768,7 @@ lemma  shift_subgoal_rr_aux4_3:"xins = Pmovq_rr (x64Syntax.RCX) (bpf_to_x64_reg 
   apply(unfold nextinstr_nf_def nextinstr_def add64_def)
   by simp
 
-lemma shift_subgoal_rr_aux4_4:"xins = Pshlq_r dst \<Longrightarrow> 
+lemma shl_subgoal_rr_aux4_4:"xins = Pshlq_r dst \<Longrightarrow> 
     Next reg' m' = (exec_instr xins 1 reg m)\<Longrightarrow> 
     \<forall> r . r \<noteq> dst \<longrightarrow> reg' (IR r) = reg (IR r)"
   apply(unfold exec_instr_def )
@@ -790,7 +776,7 @@ lemma shift_subgoal_rr_aux4_4:"xins = Pshlq_r dst \<Longrightarrow>
   apply(unfold nextinstr_nf_def nextinstr_def add64_def)
   by auto
 
-lemma  shift_subgoal_rr_aux4_5:"xins = Pshlq_r (bpf_to_x64_reg dst) \<Longrightarrow> 
+lemma  shl_subgoal_rr_aux4_5:"xins = Pshlq_r (bpf_to_x64_reg dst) \<Longrightarrow> 
     Next reg' m' = (exec_instr xins 1 reg m)\<Longrightarrow> 
     \<forall> r \<noteq> dst. reg' (IR (bpf_to_x64_reg r)) = reg (IR (bpf_to_x64_reg r))"
   apply(unfold exec_instr_def )
@@ -798,8 +784,7 @@ lemma  shift_subgoal_rr_aux4_5:"xins = Pshlq_r (bpf_to_x64_reg dst) \<Longrighta
   apply(unfold nextinstr_nf_def nextinstr_def add64_def)
   by simp
 
-
-lemma  shift_subgoal_rr_aux4_8:"xins = Ppushl_r x64Syntax.RCX \<Longrightarrow> 
+lemma  shl_subgoal_rr_aux4_6:"xins = Ppushl_r x64Syntax.RCX \<Longrightarrow> 
     Next reg' m' = (exec_instr xins 1 reg m)\<Longrightarrow> 
     \<forall> r. r \<notin> {(bpf_to_x64_reg dst), x64Syntax.RCX, x64Syntax.RSP} \<longrightarrow> reg' (IR r) = reg (IR r)"
   apply(unfold exec_instr_def )
@@ -826,8 +811,7 @@ subgoal for x5a apply(cases "storev M32 m (Vlong (x5 - x5a)) (reg (IR ireg.RCX))
   done
   done
 
-
-lemma  shift_subgoal_rr_aux4_9:"xins = Ppopl x64Syntax.RCX \<Longrightarrow> 
+lemma  shl_subgoal_rr_aux4_7:"xins = Ppopl x64Syntax.RCX \<Longrightarrow> 
     Next reg' m' = (exec_instr xins 1 reg m)\<Longrightarrow> 
     \<forall> r. r \<notin> {(bpf_to_x64_reg dst), x64Syntax.RCX, x64Syntax.RSP} \<longrightarrow> reg' (IR r) = reg (IR r)"
   apply(unfold exec_instr_def )
@@ -836,82 +820,295 @@ lemma  shift_subgoal_rr_aux4_9:"xins = Ppopl x64Syntax.RCX \<Longrightarrow>
   apply(cases "loadv M32 m (reg (IR SP))",simp_all)
   done
 
+subsubsection   \<open> BPF_ALU64 RSH aux \<close>
 
-lemma shift_subgoal_rr_aux4_6:
-  assumes a0:"xins = [Ppushl_r x64Syntax.RCX, Pmovq_rr (x64Syntax.RCX)(bpf_to_x64_reg src),Pshlq_r (bpf_to_x64_reg dst),Ppopl x64Syntax.RCX]" and 
+lemma shr_subgoal_rr_aux2_2:"xins = Pshrq_r dst \<Longrightarrow> 
+    Next reg'' m'' = (exec_instr xins 1 reg m) \<Longrightarrow> m'' = m"
+  apply(unfold exec_instr_def) by simp
+
+lemma shr_subgoal_rr_aux2_3:
+  assumes a0:"xins = [(Pmovq_rr (x64Syntax.RCX) src),(Pshrq_r dst)]" and 
+    a1:"Next reg' m' = (exec_instr (xins!0) 1 reg m) " and
+    a2:"Next reg'' m'' = (exec_instr (xins!1) 1 reg' m') " 
+  shows " m'' = m"
+  using shl_subgoal_rr_aux2_1 shr_subgoal_rr_aux2_2 
+  by (metis One_nat_def a0 a1 a2 nth_Cons_0 nth_Cons_Suc)
+
+lemma shr_subgoal_rr_aux2:
+  assumes a0:"xins = [(Pmovq_rr (x64Syntax.RCX) src),(Pshrq_r dst)]" and 
+    a1:"Next reg'' m'' = interp3 xins (Next reg m) " 
+  shows " m'' = m"
+proof-
+  have b0:"length xins = (2::nat)" using a0 by simp
+  thus ?thesis using b0 a0 a1 shr_subgoal_rr_aux2_3 
+    by (meson interp3_length2_aux2)
+qed
+
+lemma shr_subgoal_rr_aux3_2:"xins = Pshrq_r (bpf_to_x64_reg dst) \<Longrightarrow> 
+    Next reg'' m'' = (exec_instr xins 1 reg m) \<Longrightarrow> reg'' (IR SP) = reg (IR SP) "
+  apply(unfold exec_instr_def reg_rsp_consist bpf_to_x64_reg_corr)
+  apply(cases xins, simp_all)
+  apply(unfold nextinstr_def reg_rsp_consist shr64_def nextinstr_nf_def reg_rsp_consist)
+  apply(cases "reg (IR (bpf_to_x64_reg dst))",simp_all)
+      apply metis
+  subgoal for x2 apply (simp add:add64_def)sorry
+  subgoal for x3 apply (simp add:add64_def) sorry
+  subgoal for x4 apply (simp add:add64_def) sorry
+  subgoal for x5 apply (simp add:add64_def) 
+    using reg_rsp_consist by blast
+  (* no dealing with VByte conversion *)
+  done
+
+lemma shr_subgoal_rr_aux3_3:
+  assumes a0:"xins = [(Pmovq_rr (x64Syntax.RCX)(bpf_to_x64_reg src)),(Pshrq_r (bpf_to_x64_reg dst))]" and 
+    a1:"Next reg' m' = (exec_instr (xins!0) 1 reg m) " and
+    a2:"Next reg'' m'' = (exec_instr (xins!1) 1 reg' m') " 
+  shows " reg'' (IR SP) = reg (IR SP) "
+  using shl_subgoal_rr_aux3_1 shr_subgoal_rr_aux3_2 reg_rsp_consist
+  by (metis One_nat_def a0 a1 a2 nth_Cons_0 nth_Cons_Suc)
+
+lemma shr_subgoal_rr_aux3:
+  assumes a0:"xins = [(Pmovq_rr (x64Syntax.RCX)(bpf_to_x64_reg src)),(Pshrq_r (bpf_to_x64_reg dst))]" and 
+    a1:"Next reg'' m'' = interp3 xins (Next reg m) " 
+  shows "reg'' (IR SP) = reg (IR SP)"
+proof-
+  have b0:"length xins = (2::nat)" using a0 by simp
+  thus ?thesis using b0 a0 a1 shr_subgoal_rr_aux3_3 
+    by (meson interp3_length2_aux2)
+qed
+
+lemma shr_subgoal_rr_aux4_1:
+  assumes a0:"xins = [Ppushl_r x64Syntax.RCX, Pmovq_rr (x64Syntax.RCX) (bpf_to_x64_reg src),Pshrq_r (bpf_to_x64_reg dst),Ppopl x64Syntax.RCX]" and 
     a1:"Next reg'' m'' = interp3 xins (Next reg m)" 
+  shows "reg'' (IR x64Syntax.RCX) = reg (IR x64Syntax.RCX)"
+proof-
+  have a3:"hd xins = Ppushl_r x64Syntax.RCX" using a0 by simp
+  have a4:"last xins = Ppopl x64Syntax.RCX" using a0 by simp
+  have b0:"(butlast(tl xins)) = [Pmovq_rr (x64Syntax.RCX) (bpf_to_x64_reg src),Pshrq_r (bpf_to_x64_reg dst)]" using a0 by simp
+  let ?midlist = "[ Pmovq_rr (x64Syntax.RCX) (bpf_to_x64_reg src) ,Pshrq_r (bpf_to_x64_reg dst)]"
+  have b1:"\<exists> reg' m'. Next reg' m' = exec_push 1 M32 m reg (reg (IR x64Syntax.RCX))" using exec_instr_def a0 
+    using a1 exec_push_def a0 
+    by (smt (verit, del_insts) instruction.simps(6295) interp3.simps(2) option.case_eq_if outcome.case(2) outcome.simps(4))
+  then obtain reg' m' where b0:"Next reg' m' = exec_push 1 M32 m reg (reg (IR x64Syntax.RCX))" by blast
+  have b2_0:"length xins = 4" using a0 by simp
+  have b2_1: "Next reg' m' = (exec_instr (xins!0) 1 reg m)" 
+    by (simp add: a0 b0 exec_instr_def)
+  have b2:"\<exists> reg2 m2. interp3 ?midlist (Next reg' m') = Next reg2 m2" using interp3_length4_aux5 b1 a0 a1 b2_0 b0 b2_1 by fastforce
+  then obtain reg2 m2 where b3:"interp3 ?midlist (Next reg' m') = Next reg2 m2" by auto
+  have b4:"m2 = m'" using shr_subgoal_rr_aux2 by (metis b3)
+  have b5:"reg' (IR SP) =  reg2 (IR SP)" using shr_subgoal_rr_aux3 b3 by metis
+  have b6:"Next reg' m' = (exec_instr (xins!0) 1 reg m) " using a0 by (simp add: b0 exec_instr_def)
+  have b7_1:"length xins \<ge> (2::nat)" using a0 by simp
+  have b7_2:"Next reg2 m2 = interp3 (butlast xins) (Next reg m)" using b3 b0 a0 by (simp add: b6)
+  have b7:"Next reg'' m'' = (exec_instr (last xins) 1 reg2 m2)" using interp3_length4_aux4 b2_0 b7_1 b7_2 by (metis a1 outcome.inject)
+  have b8:"Next reg'' m'' = (exec_instr (last xins) 1 reg2 m')" using b7 b4 by simp
+  thus ?thesis using a3 a4 b4 b5 b6 b8 a1 push_pop_subgoal_rr_aux2_3
+    by (metis a0 b3 butlast.simps(2) list.distinct(1) list.sel(3))
+qed
+
+lemma shr_subgoal_rr_aux4_4:"xins = Pshrq_r dst \<Longrightarrow> 
+    Next reg' m' = (exec_instr xins 1 reg m)\<Longrightarrow> 
+    \<forall> r . r \<noteq> dst \<longrightarrow> reg' (IR r) = reg (IR r)"
+  apply(unfold exec_instr_def )
+  apply(cases xins, simp_all)
+  apply(unfold nextinstr_nf_def nextinstr_def add64_def)
+  by auto
+
+lemma  shr_subgoal_rr_aux4_5:"xins = Pshrq_r (bpf_to_x64_reg dst) \<Longrightarrow> 
+    Next reg' m' = (exec_instr xins 1 reg m)\<Longrightarrow> 
+    \<forall> r \<noteq> dst. reg' (IR (bpf_to_x64_reg r)) = reg (IR (bpf_to_x64_reg r))"
+  apply(unfold exec_instr_def )
+  apply(cases xins, simp_all)
+  apply(unfold nextinstr_nf_def nextinstr_def add64_def)
+  by simp
+
+subsubsection   \<open> BPF_ALU64 ARSH aux \<close>
+
+lemma sar_subgoal_rr_aux2_2:"xins = Psarq_r dst \<Longrightarrow> 
+    Next reg'' m'' = (exec_instr xins 1 reg m) \<Longrightarrow> m'' = m"
+  apply(unfold exec_instr_def) by simp
+
+lemma sar_subgoal_rr_aux2_3:
+  assumes a0:"xins = [(Pmovq_rr (x64Syntax.RCX) src),(Psarq_r dst)]" and 
+    a1:"Next reg' m' = (exec_instr (xins!0) 1 reg m) " and
+    a2:"Next reg'' m'' = (exec_instr (xins!1) 1 reg' m') " 
+  shows " m'' = m"
+  using shl_subgoal_rr_aux2_1 sar_subgoal_rr_aux2_2 
+  by (metis One_nat_def a0 a1 a2 nth_Cons_0 nth_Cons_Suc)
+
+lemma sar_subgoal_rr_aux2:
+  assumes a0:"xins = [(Pmovq_rr (x64Syntax.RCX) src),(Psarq_r dst)]" and 
+    a1:"Next reg'' m'' = interp3 xins (Next reg m) " 
+  shows " m'' = m"
+proof-
+  have b0:"length xins = (2::nat)" using a0 by simp
+  thus ?thesis using b0 a0 a1 sar_subgoal_rr_aux2_3 
+    by (meson interp3_length2_aux2)
+qed
+
+lemma sar_subgoal_rr_aux3_2:"xins = Psarq_r (bpf_to_x64_reg dst) \<Longrightarrow> 
+    Next reg'' m'' = (exec_instr xins 1 reg m) \<Longrightarrow> reg'' (IR SP) = reg (IR SP) "
+  apply(unfold exec_instr_def reg_rsp_consist bpf_to_x64_reg_corr)
+  apply(cases xins, simp_all)
+  apply(unfold nextinstr_def reg_rsp_consist shr64_def nextinstr_nf_def reg_rsp_consist)
+  apply(cases "reg (IR (bpf_to_x64_reg dst))",simp_all)
+      apply(unfold add64_def sar64_def,simp_all)
+      apply (cases  Vundef, simp_all)
+      apply(cases "reg RIP",simp_all)
+  sorry
+  (* no dealing with VByte conversion *)
+  done
+
+lemma sar_subgoal_rr_aux3_3:
+  assumes a0:"xins = [(Pmovq_rr (x64Syntax.RCX)(bpf_to_x64_reg src)),(Psarq_r (bpf_to_x64_reg dst))]" and 
+    a1:"Next reg' m' = (exec_instr (xins!0) 1 reg m) " and
+    a2:"Next reg'' m'' = (exec_instr (xins!1) 1 reg' m') " 
+  shows " reg'' (IR SP) = reg (IR SP) "
+  using shl_subgoal_rr_aux3_1 sar_subgoal_rr_aux3_2 reg_rsp_consist
+  by (metis One_nat_def a0 a1 a2 nth_Cons_0 nth_Cons_Suc)
+
+lemma sar_subgoal_rr_aux3:
+  assumes a0:"xins = [(Pmovq_rr (x64Syntax.RCX)(bpf_to_x64_reg src)),(Psarq_r (bpf_to_x64_reg dst))]" and 
+    a1:"Next reg'' m'' = interp3 xins (Next reg m) " 
+  shows "reg'' (IR SP) = reg (IR SP)"
+proof-
+  have b0:"length xins = (2::nat)" using a0 by simp
+  thus ?thesis using b0 a0 a1 sar_subgoal_rr_aux3_3 
+    by (meson interp3_length2_aux2)
+qed
+
+lemma sar_subgoal_rr_aux4_1:
+  assumes a0:"xins = [Ppushl_r x64Syntax.RCX, Pmovq_rr (x64Syntax.RCX) (bpf_to_x64_reg src),Psarq_r (bpf_to_x64_reg dst),Ppopl x64Syntax.RCX]" and 
+    a1:"Next reg'' m'' = interp3 xins (Next reg m)" 
+  shows "reg'' (IR x64Syntax.RCX) = reg (IR x64Syntax.RCX)"
+proof-
+  have a3:"hd xins = Ppushl_r x64Syntax.RCX" using a0 by simp
+  have a4:"last xins = Ppopl x64Syntax.RCX" using a0 by simp
+  have b0:"(butlast(tl xins)) = [Pmovq_rr (x64Syntax.RCX) (bpf_to_x64_reg src),Psarq_r (bpf_to_x64_reg dst)]" using a0 by simp
+  let ?midlist = "[ Pmovq_rr (x64Syntax.RCX) (bpf_to_x64_reg src) ,Psarq_r (bpf_to_x64_reg dst)]"
+  have b1:"\<exists> reg' m'. Next reg' m' = exec_push 1 M32 m reg (reg (IR x64Syntax.RCX))" using exec_instr_def a0 
+    using a1 exec_push_def a0 
+    by (smt (verit, del_insts) instruction.simps(6295) interp3.simps(2) option.case_eq_if outcome.case(2) outcome.simps(4))
+  then obtain reg' m' where b0:"Next reg' m' = exec_push 1 M32 m reg (reg (IR x64Syntax.RCX))" by blast
+  have b2_0:"length xins = 4" using a0 by simp
+  have b2_1: "Next reg' m' = (exec_instr (xins!0) 1 reg m)" 
+    by (simp add: a0 b0 exec_instr_def)
+  have b2:"\<exists> reg2 m2. interp3 ?midlist (Next reg' m') = Next reg2 m2" using interp3_length4_aux5 b1 a0 a1 b2_0 b0 b2_1 by fastforce
+  then obtain reg2 m2 where b3:"interp3 ?midlist (Next reg' m') = Next reg2 m2" by auto
+  have b4:"m2 = m'" using sar_subgoal_rr_aux2 by (metis b3)
+  have b5:"reg' (IR SP) =  reg2 (IR SP)" using sar_subgoal_rr_aux3 b3 by metis
+  have b6:"Next reg' m' = (exec_instr (xins!0) 1 reg m) " using a0 by (simp add: b0 exec_instr_def)
+  have b7_1:"length xins \<ge> (2::nat)" using a0 by simp
+  have b7_2:"Next reg2 m2 = interp3 (butlast xins) (Next reg m)" using b3 b0 a0 by (simp add: b6)
+  have b7:"Next reg'' m'' = (exec_instr (last xins) 1 reg2 m2)" using interp3_length4_aux4 b2_0 b7_1 b7_2 by (metis a1 outcome.inject)
+  have b8:"Next reg'' m'' = (exec_instr (last xins) 1 reg2 m')" using b7 b4 by simp
+  thus ?thesis using a3 a4 b4 b5 b6 b8 a1 push_pop_subgoal_rr_aux2_3
+    by (metis a0 b3 butlast.simps(2) list.distinct(1) list.sel(3))
+qed
+
+lemma sar_subgoal_rr_aux4_4:"xins = Psarq_r dst \<Longrightarrow> 
+    Next reg' m' = (exec_instr xins 1 reg m)\<Longrightarrow> 
+    \<forall> r . r \<noteq> dst \<longrightarrow> reg' (IR r) = reg (IR r)"
+  apply(unfold exec_instr_def )
+  apply(cases xins, simp_all)
+  apply(unfold nextinstr_nf_def nextinstr_def add64_def)
+  by auto
+
+lemma  sar_subgoal_rr_aux4_5:"xins = Psarq_r (bpf_to_x64_reg dst) \<Longrightarrow> 
+    Next reg' m' = (exec_instr xins 1 reg m)\<Longrightarrow> 
+    \<forall> r \<noteq> dst. reg' (IR (bpf_to_x64_reg r)) = reg (IR (bpf_to_x64_reg r))"
+  apply(unfold exec_instr_def )
+  apply(cases xins, simp_all)
+  apply(unfold nextinstr_nf_def nextinstr_def add64_def)
+  by simp
+
+subsubsection   \<open> BPF_ALU64 shift \<close>
+
+lemma shift_subgoal_rr_aux4_8:
+  assumes a0:"xins = [Ppushl_r x64Syntax.RCX, Pmovq_rr (x64Syntax.RCX)(bpf_to_x64_reg src),op (bpf_to_x64_reg dst),Ppopl x64Syntax.RCX]" and 
+    a1:"Next reg'' m'' = interp3 xins (Next reg m)" and
+    a2: "op \<in> {Pshrq_r, Pshlq_r, Psarq_r}"
   shows "\<forall> r . bpf_to_x64_reg r \<notin> {(bpf_to_x64_reg dst), x64Syntax.RCX, x64Syntax.RSP} \<longrightarrow> reg'' (IR (bpf_to_x64_reg r )) = reg (IR (bpf_to_x64_reg r ))"
 proof-
+  have b0_0:"length xins = 4" using a0 by simp
   have b0_1:"\<exists> reg1 m1. Next reg1 m1 = (exec_instr (xins!0) 1 reg m)" using exec_instr_def a0
-    by (metis a1 interp3_aux2 list.distinct(1) outcome.exhaust)
+    by (metis a1 interp3_list_aux1 list.distinct(1) outcome.exhaust)
   have b0_2:"length xins >0" using a0 by simp
   have b0_3:"\<exists> reg1 m1. Next reg1 m1 = (exec_instr (xins!0) 1 reg m) \<and> Next reg'' m'' = interp3 (tl xins) (Next reg1 m1) " 
        using a1 by (metis b0_1 b0_2 interp3.elims length_greater_0_conv list.sel(3) nth_Cons_0 outcome.case(1))
   then obtain reg1 m1 where b0_4:" Next reg1 m1 = (exec_instr (xins!0) 1 reg m) \<and> Next reg'' m'' = interp3 (tl xins) (Next reg1 m1)" by auto
-  have b0:"\<forall> r . r \<notin> {(bpf_to_x64_reg dst), x64Syntax.RCX, x64Syntax.RSP} \<longrightarrow> reg1 (IR r) = reg (IR r)" using a0 b0_2 shift_subgoal_rr_aux4_8
+  have b0:"\<forall> r . r \<notin> {(bpf_to_x64_reg dst), x64Syntax.RCX, x64Syntax.RSP} \<longrightarrow> reg1 (IR r) = reg (IR r)" using a0 b0_2 shl_subgoal_rr_aux4_6
     by (metis b0_4 nth_Cons_0)
   have b1_1:"\<exists> reg2 m2. Next reg2 m2 = (exec_instr (xins!1) 1 reg1 m1)" using exec_instr_def a0 by simp
   then obtain reg2 m2 where b1_2:"Next reg2 m2 = (exec_instr (xins!1) 1 reg1 m1)" using b1_1 by auto
   have b1_3:"take 2 xins = [xins!0]@[xins!1]" by (simp add: a0 numeral_2_eq_2 take_Suc_conv_app_nth)
   have b1_4:"Next reg2 m2 = interp3 (take 2 xins) (Next reg m)" using a0 b1_2 b1_3 b0_4
-    by (metis append_Cons append_Nil interp3.simps(2) interp3_aux4 outcome.case(1))
-  have b1_5:"[xins!0]@[xins!1] @ (drop 2 xins)= xins" using a0
-    by (simp add: Cons_nth_drop_Suc numeral_3_eq_3 numeral_nat(2))
-  have b1_6:"interp3 (drop 2 xins) (Next reg2 m2) = interp3 (xins) (Next reg m)" using a0 a1 b1_5 b1_4
-       using append_Cons append_Nil interp3.simps(2) outcome.simps(4) by (metis b0_4 b1_2)
+    by (metis append_Cons append_Nil interp3.simps(2) interp3_list_aux3 outcome.case(1))
+  have b1_5:" Next reg2 m2 = interp3 (take 2 xins) (Next reg m) \<and> Next reg'' m'' = interp3 (drop 2 xins) (Next reg2 m2)" using interp3_length4_aux4 b0_0 a1 b1_4 by metis
   have b1:"\<forall> r . r \<notin> {(bpf_to_x64_reg dst), x64Syntax.RCX} \<longrightarrow> reg1 (IR r) = reg2 (IR r)" using a0 b1_2
-    by (metis One_nat_def insertCI nth_Cons_0 nth_Cons_Suc shift_subgoal_rr_aux4_2)
+    by (metis One_nat_def insertCI nth_Cons_0 nth_Cons_Suc shl_subgoal_rr_aux4_2)
   have b2_1:"\<exists> reg3 m3. Next reg3 m3 = (exec_instr (xins!2) 1 reg2 m2)" 
-    by (simp add: a0 exec_instr_def)
+    using a0 a2 exec_instr_def by auto
   then obtain reg3 m3 where b2_2:"Next reg3 m3 = (exec_instr (xins!2) 1 reg2 m2)" using b1_1 by auto
   have b2_3:"take 3 xins = [xins!0]@[xins!1]@[xins!2]" using a0 
     by (simp add: One_nat_def Suc_1 add_One numeral_3_eq_3 numeral_nat(2) take_Suc_conv_app_nth)
-  have b2_4:"Next reg3 m3 = interp3 (take 3 xins) (Next reg m)" using a0 b1_6 b2_3 b2_2
-    using append_Cons append_Nil b0_4 b1_2 b1_4 interp3.simps(2) interp3_aux4 outcome.case(1) by metis
+  have b2_4:"Next reg3 m3 = interp3 (take 3 xins) (Next reg m)" using a0 b1_5 b2_3 b2_2
+    using append_Cons append_Nil b0_4 b1_2 b1_4 interp3.simps(2) interp3_list_aux3 outcome.case(1) by metis
   have b2_5:"[xins!0]@[xins!1]@[xins!2]@[last xins] = xins" using append_butlast_last_id a0 by fastforce
   have b2_6:"(last xins) = (xins!3)" using a0 by (metis One_nat_def Suc_eq_plus1 Suc_numeral add_2_eq_Suc diff_Suc_1' last_conv_nth length_Suc_conv list.simps(3) list.size(3) list_consists_4 semiring_norm(5))
   have b2_7: "(butlast xins) = [xins!0]@[xins!1]@[xins!2]" using a0 b2_6 by simp
   have b2_8:"butlast xins = take 3 xins" using a0 b2_7 by simp
-  have b2_9:"Next reg3 m3 = interp3 (take 3 xins) (Next reg m) \<and> Next reg'' m'' = (exec_instr (last xins) 1 reg3 m3)" using a0 
-    by (smt (verit, ccfv_threshold) One_nat_def Suc_eq_plus1 a1 append_Cons append_Nil b1_5 b1_6 b2_2 b2_4 b2_5 interp3_aux5 list.size(3) list.size(4) nat_1_add_1 nth_Cons_0 nth_Cons_Suc outcome.inject same_append_eq)
+  have b2_9:"Next reg3 m3 = interp3 (butlast xins) (Next reg m) \<and> Next reg'' m'' = (exec_instr (last xins) 1 reg3 m3)" using a0 b2_4 b2_8 interp3_length4_aux4 b0_0 a1 sorry(* by (metis a1 outcome.inject)*)
+  have b2_10:"Next reg3 m3 = interp3 (take 3 xins) (Next reg m) \<and> Next reg'' m'' = (exec_instr (last xins) 1 reg3 m3)" using b2_9 b2_8 by simp
   have b2:"\<forall> r . r \<notin> {(bpf_to_x64_reg dst), x64Syntax.RCX} \<longrightarrow> reg3 (IR r) = reg2 (IR r)" using a0 b1_2
-    using b2_2 shift_subgoal_rr_aux4_4 by auto
+    using b2_2 shr_subgoal_rr_aux4_4 shl_subgoal_rr_aux4_4 sar_subgoal_rr_aux4_4 a2 by auto
   hence b3_1:" \<exists> reg4 m4. Next reg4 m4 = (exec_instr (xins!3) 1 reg3 m3)" 
     using b2_6 b2_9 by auto
   then obtain reg4 m4 where b4:"Next reg4 m4 = (exec_instr (xins!3) 1 reg3 m3)" using b3_1 by auto
-  have b3:"Next reg4 m4 = Next reg'' m''" using interp3_aux4
+  have b3:"Next reg4 m4 = Next reg'' m''" using interp3_list_aux3
     by (simp add: b2_6 b2_9 b4)
-  have b4:"\<forall> r . r \<notin> {(bpf_to_x64_reg dst), x64Syntax.RCX, x64Syntax.RSP} \<longrightarrow> reg3 (IR r) = reg'' (IR r)" using a0 b0 b1 b2 shift_subgoal_rr_aux4_9 
+  have b4:"\<forall> r . r \<notin> {(bpf_to_x64_reg dst), x64Syntax.RCX, x64Syntax.RSP} \<longrightarrow> reg3 (IR r) = reg'' (IR r)" using a0 b0 b1 b2 shl_subgoal_rr_aux4_7 
     by (metis append_Cons append_Nil b2_5 b2_9 list.sel(1) list.sel(3))
   thus ?thesis using b0 b1 b2 b3 by simp
 qed
 
 lemma shift_subgoal_rr_aux4:
-  assumes a0:"xins = [Ppushl_r x64Syntax.RCX, Pmovq_rr (x64Syntax.RCX) (bpf_to_x64_reg src) ,Pshlq_r (bpf_to_x64_reg dst),Ppopl x64Syntax.RCX] " and
-    a1:"Next reg'' m'' = interp3 xins (Next reg m) " 
-  shows" \<forall> r \<noteq> dst. reg'' (IR  (bpf_to_x64_reg r)) = reg (IR (bpf_to_x64_reg r))"
+  assumes a0:"xins = [Ppushl_r x64Syntax.RCX, Pmovq_rr (x64Syntax.RCX) (bpf_to_x64_reg src) ,op (bpf_to_x64_reg dst),Ppopl x64Syntax.RCX] " and
+    a1:"Next reg'' m'' = interp3 xins (Next reg m) " and
+    a2: "op \<in> {Pshrq_r, Pshlq_r, Psarq_r}"
+  shows" \<forall> r \<noteq> dst. reg'' (IR  (bpf_to_x64_reg r)) = reg (IR (bpf_to_x64_reg r))" 
 proof-
-  have b0:"reg'' (IR x64Syntax.RCX) = reg (IR x64Syntax.RCX)" using a0 a1 shift_subgoal_rr_aux4_1 by simp
-  have b1:"\<forall> r . bpf_to_x64_reg r  \<notin> {(bpf_to_x64_reg dst), x64Syntax.RCX, x64Syntax.RSP} \<longrightarrow> reg'' (IR (bpf_to_x64_reg r )) = reg (IR (bpf_to_x64_reg r ))" using shift_subgoal_rr_aux4_6 a0 a1 by simp
+  have b0:"reg'' (IR x64Syntax.RCX) = reg (IR x64Syntax.RCX)" using a0 a1 a2 shl_subgoal_rr_aux4_1 shr_subgoal_rr_aux4_1 sar_subgoal_rr_aux4_1 by auto
+  have b1:"\<forall> r . bpf_to_x64_reg r  \<notin> {(bpf_to_x64_reg dst), x64Syntax.RCX, x64Syntax.RSP} \<longrightarrow> reg'' (IR (bpf_to_x64_reg r )) = reg (IR (bpf_to_x64_reg r ))" using shift_subgoal_rr_aux4_8 a0 a1 a2 by auto
   have b1_1:"\<forall> r. (bpf_to_x64_reg r) \<noteq> x64Syntax.RSP" using a0 reg_rsp_consist by simp
   thus ?thesis using  b0 b1 b1_1  by force
 qed
 
-(*lemma shift_subgoal_rr_aux5_1:
+(*lemma shl_subgoal_rr_aux5_1:
      "bins = BPF_ALU64 BPF_LSH dst (SOReg src) \<Longrightarrow>
-     xins = [Ppushl_r x64Syntax.RCX, Pmovq_rr (x64Syntax.RCX) ri,Pshlq_r rd,Ppopl x64Syntax.RCX] \<Longrightarrow>
+     xins = Pshlq_r rd \<Longrightarrow>
      (BPF_OK pc rs' m' ss' is_v1 (cur_cu+1) remain_cu) = step fuel bins rs m ss is_v1 cur_cu remain_cu \<Longrightarrow>
-     Next reg' m' = interp3 xins (Next reg m) \<Longrightarrow>
+     Next reg' m' = exec_instr xins sz reg m \<Longrightarrow>
      rd = (bpf_to_x64_reg dst) \<Longrightarrow>
-     ri = (bpf_to_x64_reg src) \<Longrightarrow>
+     x64Syntax.RCX = (bpf_to_x64_reg src) \<Longrightarrow>
      reg (IR rd) = Vlong n1 \<Longrightarrow>
      reg (IR ri) = Vlong n2 \<Longrightarrow>
      n1  = rs dst \<Longrightarrow>
      n2  = rs src \<Longrightarrow> 
      Vlong (rs' dst) = reg' (IR (bpf_to_x64_reg dst))"
-  sorry
-*)
-lemma shift_subgoal_rr_aux5:
+  apply(unfold exec_instr_def)
+  apply(cases xins,simp_all)
+  subgoal for x46 apply(cases is_v1,simp_all)
+     apply(cases "eval_alu64 BPF_LSH dst (SOReg src) rs enable_instruction_meter",simp_all)
+     apply(unfold nextinstr_nf_def nextinstr_def add64_def shl64_def eval_alu64_def,simp_all)
+     apply(cases "reg (IR ireg.RCX)",simp_all)
+         apply(unfold eval_alu64_aux2_def Let_def eval_reg_def)
+         apply(cases BPF_LSH,simp_all)
+         apply(cases "reg RIP",simp_all)
+    sorry
+  done
+ *)
+lemma shl_subgoal_rr_aux5:
   assumes a0:"bins = BPF_ALU64 BPF_LSH dst (SOReg src)" and
      a1:"xins = [Ppushl_r x64Syntax.RCX, Pmovq_rr (x64Syntax.RCX) ri,Pshlq_r rd,Ppopl x64Syntax.RCX]" and
      a2:"(BPF_OK pc rs' m' ss' is_v1 (cur_cu+1) remain_cu) = step fuel bins rs m ss is_v1 cur_cu remain_cu" and
@@ -925,43 +1122,14 @@ lemma shift_subgoal_rr_aux5:
      a9:"(bpf_to_x64_reg dst) \<noteq> x64Syntax.RCX"
      shows "Vlong (rs' dst) = reg' (IR (bpf_to_x64_reg dst))"
   sorry
+  done
 
-lemma shift_subgoal_rr_aux6:"
+lemma shl_subgoal_rr_aux6:"
     bins = BPF_ALU64 BPF_LSH dst (SOReg src) \<Longrightarrow> (BPF_OK pc rs' m' ss' is_v1 (cur_cu+1) remain_cu) = step fuel bins rs m ss is_v1 cur_cu remain_cu \<Longrightarrow>
     \<forall> r \<noteq> dst. rs' r = rs r"
   apply(cases "bins",simp_all)
   apply(unfold eval_alu64_def,simp)
   by (unfold eval_alu64_aux2_def, simp_all)
-
-lemma test1:
-  assumes 
-       a1:"Some bl = x64_encode (Porq_rr dst src)" and
-       a2:"list_in_list bl (unat pc) l_bin" and
-       a3:"x64_decode (unat pc) l_bin = Some (length l_bin, xins)"  
-     shows "xins = Porq_rr dst src"
-  using x64_encode_decode_consistency 
-  by (metis a1 a2 a3 option.sel prod.inject)
-
-value "x64_decodes 0 (Option.the(x64_encodes_suffix ([Pmovq_rr x64Syntax.RAX x64Syntax.RBX,Pnop])))"
-value "x64_decodes 0 (Option.the(x64_encodes_suffix ([Pnop,Pnop])))"
-value "map snd [(1::nat,Pnop),(3::nat,Pmovq_rr x64Syntax.RAX x64Syntax.RBX)]"
-
-
-value "x64_encodes_suffix [Pmovq_rr src dst,Pmovq_rr src dst]"
-value "x64_decodes 0 (Option.the(x64_encodes_suffix [Ppushl_r x64Syntax.RCX, Pmovq_rr (x64Syntax.RAX) (x64Syntax.RCX),
-  Pshlq_r (x64Syntax.RBX),Ppopl x64Syntax.RCX]))"
-value "x64_decodes 0 (Option.the(x64_encodes_suffix [Ppushl_r x64Syntax.RCX, Pmovq_rr (bpf_to_x64_reg src) (x64Syntax.RCX),
-Pshlq_r (bpf_to_x64_reg dst),Ppopl x64Syntax.RCX]))"
-
-lemma test2:
-  assumes 
-       a1:"Some bl = x64_encodes_suffix [Pnop]" and
-       a2:"list_in_list bl 0 l_bin" and
-       a3:"x64_decodes 0 l_bin = Some v" and
-       a4:"xins = map snd v"  
-     shows "xins = [Pnop]"
-  using x64_encodes_decodes_consistency a1 a2 a3 a4 by simp
-
 
 lemma shlq_subgoal_rr_generic:
   assumes a0:"bins = BPF_ALU64 BPF_LSH dst (SOReg src)" and
@@ -982,17 +1150,163 @@ proof -
     using a8 calculation by presburger
     moreover have b1:"Vlong (rs dst) = reg (IR (bpf_to_x64_reg dst))" using a6 spec by simp
     moreover have b2:"Vlong (rs src) = reg (IR (bpf_to_x64_reg src))" using a6 spec by simp
-    hence b3:"Vlong (rs' dst) = reg' (IR (bpf_to_x64_reg dst))" using shift_subgoal_rr_aux5 b0 b1 b2 a0 a4 a5 by force
+    hence b3:"Vlong (rs' dst) = reg' (IR (bpf_to_x64_reg dst))" using shl_subgoal_rr_aux5 b0 b1 b2 a0 a4 a5 by (metis a7)
     have b4:"\<forall> r \<noteq> dst. reg'(IR (bpf_to_x64_reg r)) = reg (IR (bpf_to_x64_reg r))" using b0 a5 shift_subgoal_rr_aux4 by simp
-    have b5:"\<forall> r \<noteq> dst. Vlong (rs' r) = Vlong (rs r)" using a0 a4 shift_subgoal_rr_aux6 by blast
+    have b5:"\<forall> r \<noteq> dst. Vlong (rs' r) = Vlong (rs r)" using a0 a4 shl_subgoal_rr_aux6 by blast
+    have b6:"\<forall> r \<noteq> dst. Vlong (rs r) = reg (IR (bpf_to_x64_reg r))" using a6 by blast
+    have b7:"(\<forall> r \<noteq> dst. Vlong (rs' r) = reg' (IR (bpf_to_x64_reg r)))" by(simp add:b4 b5 b6) 
+    thus ?thesis using b3 by fastforce
+  qed
+
+(*lemma shr_subgoal_rr_aux5_1:
+     "bins = BPF_ALU64 BPF_RSH dst (SOReg src) \<Longrightarrow>
+     xins = Pshrq_r rd \<Longrightarrow>
+     (BPF_OK pc rs' m' ss' is_v1 (cur_cu+1) remain_cu) = step fuel bins rs m ss is_v1 cur_cu remain_cu \<Longrightarrow>
+     Next reg' m' = exec_instr xins sz reg m \<Longrightarrow>
+     rd = (bpf_to_x64_reg dst) \<Longrightarrow>
+     x64Syntax.RCX = (bpf_to_x64_reg src) \<Longrightarrow>
+     reg (IR rd) = Vlong n1 \<Longrightarrow>
+     reg (IR ri) = Vlong n2 \<Longrightarrow>
+     n1  = rs dst \<Longrightarrow>
+     n2  = rs src \<Longrightarrow> 
+     Vlong (rs' dst) = reg' (IR (bpf_to_x64_reg dst))"
+  apply(unfold exec_instr_def)
+  apply(cases xins,simp_all)
+  subgoal for x46 apply(cases is_v1,simp_all)
+     apply(cases "eval_alu64 BPF_RSH dst (SOReg src) rs enable_instruction_meter",simp_all)
+     apply(unfold nextinstr_nf_def nextinstr_def add64_def shl64_def eval_alu64_def,simp_all)
+     apply(cases "reg (IR ireg.RCX)",simp_all)
+         apply(unfold eval_alu64_aux2_def Let_def eval_reg_def)
+         apply(cases BPF_RSH,simp_all)
+         apply(cases "reg RIP",simp_all)
+    sorry
+  done
+*)
+lemma shr_subgoal_rr_aux5:
+  assumes a0:"bins = BPF_ALU64 BPF_RSH dst (SOReg src)" and
+     a1:"xins = [Ppushl_r x64Syntax.RCX, Pmovq_rr (x64Syntax.RCX) ri,Pshrq_r rd,Ppopl x64Syntax.RCX]" and
+     a2:"(BPF_OK pc rs' m' ss' is_v1 (cur_cu+1) remain_cu) = step fuel bins rs m ss is_v1 cur_cu remain_cu" and
+     a3:"Next reg' m' = interp3 xins (Next reg m)" and
+     a4:"rd = (bpf_to_x64_reg dst)" and
+     a5:"ri = (bpf_to_x64_reg src)" and
+     a6:"reg (IR rd) = Vlong n1" and
+     a7:"reg (IR ri) = Vlong n2" and
+     a8:"n1  = rs dst" and
+     a9:"n2  = rs src" and
+     a9:"(bpf_to_x64_reg dst) \<noteq> x64Syntax.RCX"
+     shows "Vlong (rs' dst) = reg' (IR (bpf_to_x64_reg dst))"
+  sorry
+
+
+lemma shr_subgoal_rr_aux6:"
+    bins = BPF_ALU64 BPF_RSH dst (SOReg src) \<Longrightarrow> (BPF_OK pc rs' m' ss' is_v1 (cur_cu+1) remain_cu) = step fuel bins rs m ss is_v1 cur_cu remain_cu \<Longrightarrow>
+    \<forall> r \<noteq> dst. rs' r = rs r"
+  apply(cases "bins",simp_all)
+  apply(unfold eval_alu64_def,simp)
+  by (unfold eval_alu64_aux2_def, simp_all)
+
+lemma shrq_subgoal_rr_generic:
+  assumes a0:"bins = BPF_ALU64 BPF_RSH dst (SOReg src)" and
+       a1:"per_jit_shift_reg64 5 dst src = Some bl" and
+       a2:"list_in_list bl (unat pc) l_bin" and
+       a3:"x64_decodes (unat pc) l_bin = Some v" and
+       a4:"(BPF_OK pc rs' m' ss' is_v1 (cur_cu+1) remain_cu) = step fuel bins rs m ss is_v1 cur_cu remain_cu" and
+       a5:"Next reg' m' = interp3 xins (Next reg m) " and
+       a6:"(\<forall> r. Vlong (rs r) = reg (IR (bpf_to_x64_reg r)))" and
+       a7:"(bpf_to_x64_reg dst) \<noteq> x64Syntax.RCX" and
+       a8:"xins = map snd v"
+  shows "(\<forall> r. Vlong (rs' r) = reg' (IR (bpf_to_x64_reg r)))"
+proof -
+  have b:"Some bl = x64_encodes_suffix [Ppushl_r x64Syntax.RCX, Pmovq_rr(x64Syntax.RCX) (bpf_to_x64_reg src),Pshrq_r (bpf_to_x64_reg dst),Ppopl x64Syntax.RCX]" 
+    using a0 a1 a7 per_jit_shift_reg64_def by simp
+  moreover have b0:"xins = [Ppushl_r x64Syntax.RCX, Pmovq_rr (x64Syntax.RCX)(bpf_to_x64_reg src),Pshrq_r (bpf_to_x64_reg dst),Ppopl x64Syntax.RCX]" 
+    using x64_encodes_decodes_consistency per_jit_shift_reg64_def a1 a2 a3 
+    using a8 calculation by presburger
+    moreover have b1:"Vlong (rs dst) = reg (IR (bpf_to_x64_reg dst))" using a6 spec by simp
+    moreover have b2:"Vlong (rs src) = reg (IR (bpf_to_x64_reg src))" using a6 spec by simp
+    hence b3:"Vlong (rs' dst) = reg' (IR (bpf_to_x64_reg dst))" using shr_subgoal_rr_aux5 b0 b1 b2 a0 a4 a5 a7 by metis
+    have b4:"\<forall> r \<noteq> dst. reg'(IR (bpf_to_x64_reg r)) = reg (IR (bpf_to_x64_reg r))" using b0 a5 shift_subgoal_rr_aux4 by simp
+    have b5:"\<forall> r \<noteq> dst. Vlong (rs' r) = Vlong (rs r)" using a0 a4 shr_subgoal_rr_aux6 by blast
+    have b6:"\<forall> r \<noteq> dst. Vlong (rs r) = reg (IR (bpf_to_x64_reg r))" using a6 by blast
+    have b7:"(\<forall> r \<noteq> dst. Vlong (rs' r) = reg' (IR (bpf_to_x64_reg r)))" by(simp add:b4 b5 b6) 
+    thus ?thesis using b3 by fastforce
+  qed
+
+(*lemma sar_subgoal_rr_aux5_1:
+     "bins = BPF_ALU64 BPF_ARSH dst (SOReg src) \<Longrightarrow>
+     xins = Pshrq_r rd \<Longrightarrow>
+     (BPF_OK pc rs' m' ss' is_v1 (cur_cu+1) remain_cu) = step fuel bins rs m ss is_v1 cur_cu remain_cu \<Longrightarrow>
+     Next reg' m' = exec_instr xins sz reg m \<Longrightarrow>
+     rd = (bpf_to_x64_reg dst) \<Longrightarrow>
+     x64Syntax.RCX = (bpf_to_x64_reg src) \<Longrightarrow>
+     reg (IR rd) = Vlong n1 \<Longrightarrow>
+     reg (IR ri) = Vlong n2 \<Longrightarrow>
+     n1  = rs dst \<Longrightarrow>
+     n2  = rs src \<Longrightarrow> 
+     Vlong (rs' dst) = reg' (IR (bpf_to_x64_reg dst))"
+  apply(unfold exec_instr_def)
+  apply(cases xins,simp_all)
+  subgoal for x46 apply(cases is_v1,simp_all)
+     apply(cases "eval_alu64 BPF_ARSH dst (SOReg src) rs enable_instruction_meter",simp_all)
+     apply(unfold nextinstr_nf_def nextinstr_def add64_def shl64_def eval_alu64_def,simp_all)
+     apply(cases "reg (IR ireg.RCX)",simp_all)
+         apply(unfold eval_alu64_aux2_def Let_def eval_reg_def)
+         apply(cases BPF_ARSH,simp_all)
+         apply(cases "reg RIP",simp_all)
+    sorry
+  done
+*)
+
+lemma sar_subgoal_rr_aux5:
+  assumes a0:"bins = BPF_ALU64 BPF_ARSH dst (SOReg src)" and
+     a1:"xins = [Ppushl_r x64Syntax.RCX, Pmovq_rr (x64Syntax.RCX) ri,Psarq_r rd,Ppopl x64Syntax.RCX]" and
+     a2:"(BPF_OK pc rs' m' ss' is_v1 (cur_cu+1) remain_cu) = step fuel bins rs m ss is_v1 cur_cu remain_cu" and
+     a3:"Next reg' m' = interp3 xins (Next reg m)" and
+     a4:"rd = (bpf_to_x64_reg dst)" and
+     a5:"ri = (bpf_to_x64_reg src)" and
+     a6:"reg (IR rd) = Vlong n1" and
+     a7:"reg (IR ri) = Vlong n2" and
+     a8:"n1  = rs dst" and
+     a9:"n2  = rs src" and
+     a9:"(bpf_to_x64_reg dst) \<noteq> x64Syntax.RCX"
+     shows "Vlong (rs' dst) = reg' (IR (bpf_to_x64_reg dst))"
+  sorry
+
+
+lemma sar_subgoal_rr_aux6:"
+    bins = BPF_ALU64 BPF_ARSH dst (SOReg src) \<Longrightarrow> (BPF_OK pc rs' m' ss' is_v1 (cur_cu+1) remain_cu) = step fuel bins rs m ss is_v1 cur_cu remain_cu \<Longrightarrow>
+    \<forall> r \<noteq> dst. rs' r = rs r"
+  apply(cases "bins",simp_all)
+  apply(unfold eval_alu64_def,simp)
+  by (unfold eval_alu64_aux3_def, simp_all)
+
+lemma sarq_subgoal_rr_generic:
+  assumes a0:"bins = BPF_ALU64 BPF_ARSH dst (SOReg src)" and
+       a1:"per_jit_shift_reg64 (7::nat) dst src = Some bl" and
+       a2:"list_in_list bl (unat pc) l_bin" and
+       a3:"x64_decodes (unat pc) l_bin = Some v" and
+       a4:"(BPF_OK pc rs' m' ss' is_v1 (cur_cu+1) remain_cu) = step fuel bins rs m ss is_v1 cur_cu remain_cu" and
+       a5:"Next reg' m' = interp3 xins (Next reg m) " and
+       a6:"(\<forall> r. Vlong (rs r) = reg (IR (bpf_to_x64_reg r)))" and
+       a7:"(bpf_to_x64_reg dst) \<noteq> x64Syntax.RCX" and
+       a8:"xins = map snd v"
+  shows "(\<forall> r. Vlong (rs' r) = reg' (IR (bpf_to_x64_reg r)))"
+proof -
+  have b:"Some bl = x64_encodes_suffix [Ppushl_r x64Syntax.RCX, Pmovq_rr(x64Syntax.RCX) (bpf_to_x64_reg src),Psarq_r (bpf_to_x64_reg dst),Ppopl x64Syntax.RCX]" 
+    using a0 a1 a7 per_jit_shift_reg64_def sorry
+  moreover have b0:"xins = [Ppushl_r x64Syntax.RCX, Pmovq_rr (x64Syntax.RCX)(bpf_to_x64_reg src),Psarq_r (bpf_to_x64_reg dst),Ppopl x64Syntax.RCX]" 
+    using x64_encodes_decodes_consistency per_jit_shift_reg64_def a1 a2 a3 
+    using a8 calculation by presburger
+    moreover have b1:"Vlong (rs dst) = reg (IR (bpf_to_x64_reg dst))" using a6 spec by simp
+    moreover have b2:"Vlong (rs src) = reg (IR (bpf_to_x64_reg src))" using a6 spec by simp
+    hence b3:"Vlong (rs' dst) = reg' (IR (bpf_to_x64_reg dst))" using sar_subgoal_rr_aux5 b0 b1 b2 a0 a4 a5 a7 by metis
+    have b4:"\<forall> r \<noteq> dst. reg'(IR (bpf_to_x64_reg r)) = reg (IR (bpf_to_x64_reg r))" using b0 a5 shift_subgoal_rr_aux4 by simp
+    have b5:"\<forall> r \<noteq> dst. Vlong (rs' r) = Vlong (rs r)" using a0 a4 sar_subgoal_rr_aux6 by blast
     have b6:"\<forall> r \<noteq> dst. Vlong (rs r) = reg (IR (bpf_to_x64_reg r))" using a6 by blast
     have b7:"(\<forall> r \<noteq> dst. Vlong (rs' r) = reg' (IR (bpf_to_x64_reg r)))" by(simp add:b4 b5 b6) 
     thus ?thesis using b3 by fastforce
   qed
 
 
-
- 
-  
 
 end
